wip

ulib/experimental/Steel.Hashtbl.fst
@@ -21,45 +21,28 @@ module Steel.Hashtbl
 
 open Steel.FractionalPermission
 open Steel.Memory
-open Steel.Effect
-open Steel.Effect.Atomic
-open Steel.Reference
+open Steel.ST.Effect.Ghost
+open Steel.ST.Effect.Atomic
+open Steel.ST.Effect
+open Steel.ST.Util
 
 module G = FStar.Ghost
 module Seq = FStar.Seq
-module Set = FStar.Set
-module Map = FStar.Map
+module Map = FStar.PartialMap
 module U32 = FStar.UInt32
-module A = Steel.Array
+module R = Steel.ST.GhostReference
+module A = Steel.ST.Array
 
 #set-options "--ide_id_info_off --print_implicits"
 
-/// We implement the table using an array of length n as the store,
-///
-/// The elements of the array are (k, v) pairs in the hashtable
-///
-/// For a key k, we would compute the index in the array as ((h k) % store.len)
-///
-/// We will then lookup the index, if it is Some (k', _) then k' == k implies that the key k is present
-///   in the table
-///
-/// We also maintain a ghost reference to store the logical map view of the hashtable
-
 noeq
-type tbl k v (h:hash_fn k) = {
+type tbl #k #v #contents (#vp:vp_t k v contents) (h:hash_fn k) (finalizer:finalizer_t vp) = {
   store_len    : n:u32{U32.v n > 0};
   store        : A.array (option (k & v));
-  g_repr       : ghost_ref (Map.t k v);
-  default_v    : G.erased v;
+  g_repr       : R.ref (Map.t k contents);
+  g_borrows    : R.ref (Map.t k v);
   store_len_pf : squash (A.length store == U32.v store_len);
 }
-
-
-/// The underlying sequence representation of the hashtable store has
-///   the following properties:
-///
-/// - Its length is bounded by u32
-/// - For a Some (k, _) entry at index i, (h k % len == i)
 
 let seq_props (#k:eqtype) (#v:Type0) (h:hash_fn k) (s:Seq.seq (option (k & v))) : prop =  
   0 < Seq.length s /\ UInt.size (Seq.length s) 32 /\
@@ -68,117 +51,93 @@ let seq_props (#k:eqtype) (#v:Type0) (h:hash_fn k) (s:Seq.seq (option (k & v))) 
                                                          U32.v (h x) `UInt.mod` Seq.length s == i))
 
 
-/// Given seq_props, we can prove that all the keys in the sequence are distinct
-///
-/// Sometimes in the proofs, it is easier to directly use the uniqueness property,
-///   rather than the seq_props
-
 let seq_keys_distinct (#k:eqtype) (#v:Type0) (s:Seq.seq (option (k & v))) : prop =
   forall (i j:(k:nat{k < Seq.length s})).{:pattern Seq.index s i; Seq.index s j}
     (i =!= j /\ Some? (Seq.index s i) /\ Some? (Seq.index s j)) ==>
     (fst (Some?.v (Seq.index s i)) =!= fst (Some?.v (Seq.index s j)))
 
-
-/// We can easily prove the distinctness property given seq_props
-
 let seq_props_implies_seq_keys_distinct (#k:eqtype) (#v:Type0) (h:hash_fn k) (s:Seq.seq (option (k & v)))
   : Lemma (requires seq_props h s) (ensures seq_keys_distinct s)
   = ()
 
-
-/// We now relate the store to the logical map
-///
-/// We first define a function to convert the sequence to a map
-///
-/// Later, we will maintain an invariant that the map obtained by applying this function
-///   to the store is a submap of the logical map
-
-let rec seq_to_map (#k:eqtype) (#v:Type0) (s:Seq.seq (option (k & v))) (default_v:v)
-  : GTot (repr k v) (decreases Seq.length s)
+let rec seq_to_map (#k:eqtype) (#v:Type0) (s:Seq.seq (option (k & v)))
+  : GTot (Map.t k v) (decreases Seq.length s)
   = if Seq.length s = 0
-    then empty_repr default_v
+    then Map.empty k v
     else let hd, tl = Seq.head s, Seq.tail s in
-         let m = seq_to_map tl default_v in
+         let m = seq_to_map tl in
          match hd with
          | None -> m
-         | Some (x, y) -> Map.upd m x y
+         | Some (x, y) -> Map.upd x y m
+
+let keys_in (#k:eqtype) (#v1 #v2:Type0) (m1:Map.t k v1) (m2:Map.t k v2) : prop =
+  let open FStar.PartialMap in
+  forall (x:k). contains x m1 ==> contains x m2
 
 let submap_of (#k:eqtype) (#v:Type0) (m1 m2:Map.t k v) : prop =
-  let open FStar.Map in
-  forall (x:k). m1 `contains` x ==> (m2 `contains` x /\ m1 `sel` x == m2 `sel` x)
-
-
-/// The main separation logic assertion
-///
-/// Maintains the permission to the store and the ghost reference,
-///   and a pure proposition to relate the two
+  let open FStar.PartialMap in
+  forall (x:k). contains x m1 ==> (contains x m2 /\ sel x m1 == sel x m2)
 
 [@@__reduce__]
-let store_contents_pred (#k:eqtype) (#v:Type0) (#h:hash_fn k) (arr:tbl k v h) (m:repr k v)
-  : Seq.lseq (option (k & v)) (A.length arr.store) -> vprop
+let store_contents_pred
+  (#k:eqtype)
+  (#v #contents:Type0)
+  (#vp:vp_t k v contents)
+  (#h:hash_fn k)
+  (#finalizer:finalizer_t vp)
+  (arr:tbl h finalizer)
+  (m:repr k contents)
+  (borrows:Map.t k v)
+  : Seq.seq (option (k & v)) -> vprop
   = fun s ->
-    A.varray_pts_to arr.store s
+    A.pts_to arr.store s
       `star`
-    ghost_pts_to arr.g_repr full_perm m
+    R.pts_to arr.g_repr full_perm m
       `star`
-    pure (seq_props h s /\ seq_to_map s arr.default_v `submap_of` m)
+    R.pts_to arr.g_borrows full_perm borrows
+      `star`
+    pure (seq_props h s /\
+          seq_to_map s `keys_in` m /\
+          borrows `submap_of` seq_to_map s)
 
 [@@__reduce__]
-let tpts_to arr m = h_exists (store_contents_pred arr m)
+let tperm arr m borrows = exists_ (store_contents_pred arr m borrows)
 
-
-/// Some pure lemmas for a few properties of the store and logical map
-
-
-let rec seq_to_map_create (k:eqtype) (#v:Type0) (n:nat) (default_v:v)
-  : Lemma (Map.equal (seq_to_map (Seq.create n None) default_v)
-                     (empty_repr #k #v default_v))
+let rec seq_to_map_create (k:eqtype) (v:Type0) (n:nat)
+  : Lemma (Map.equal (seq_to_map (Seq.create n None))
+                     (Map.empty k v))
   = if n = 0 then ()
     else begin
       assert (Seq.equal #(option (k & v)) (Seq.tail (Seq.create n None))
                                           (Seq.create (n-1) None));
-      seq_to_map_create k (n-1) default_v
+      seq_to_map_create k v (n-1)
     end
 
-
-/// The ith entry in the sequence, if it is Some (x, y) then in the corresponding map x |-> v
-///
-/// Note that this needs that the keys in the sequence are distinct
-
-let rec seq_to_map_ith (#k:eqtype) (#v:Type0) (s:Seq.seq (option (k & v))) (default_v:v)
-  (i:nat{i < Seq.length s})
+let rec seq_to_map_ith (#k:eqtype) (#v:Type0) (s:Seq.seq (option (k & v))) (i:nat{i < Seq.length s})
   : Lemma
       (requires
         seq_keys_distinct s /\
         Some? (Seq.index s i))
       (ensures (let open Map in
                 let Some (x, y) = Seq.index s i in
-                let m = seq_to_map s default_v in
-                m `contains` x /\
-                m `sel` x == y))
+                let m = seq_to_map s in
+                contains x m /\
+                sel x m == Some y))
       (decreases i)
-  = if i = 0 then () else seq_to_map_ith (Seq.tail s) default_v (i-1)
+  = if i = 0 then () else seq_to_map_ith (Seq.tail s) (i-1)
 
-
-/// The domain of the seq_to_map map is strictly the entries in the sequence
-
-let rec seq_to_map_domain (#k:eqtype) (#v:Type0) (s:Seq.seq (option (k & v))) (default_v:v) (x:k)
+let rec seq_to_map_domain (#k:eqtype) (#v:Type0) (s:Seq.seq (option (k & v))) (x:k)
   : Lemma
       (ensures
-        seq_to_map s default_v `Map.contains` x ==>  //if x is in the seq_to_map map,
+        Map.contains x (seq_to_map s) ==>  //if x is in the seq_to_map map,
         (exists (i:nat{i < Seq.length s}).
            Some? (Seq.index s i) /\
            fst (Some?.v (Seq.index s i)) == x))  //then it must be in the sequence
       (decreases Seq.length s)
   = if Seq.length s = 0 then ()
-    else seq_to_map_domain (Seq.tail s) default_v x
+    else seq_to_map_domain (Seq.tail s) x
 
-
-/// Commutation of seq_to_map with Seq.upd
-///
-/// It requires the keys distinctness property in the original and updated sequence
-
-let rec seq_to_map_upd (#k:eqtype) (#v:Type0) (s:Seq.seq (option (k & v))) (default_v:v)
+let rec seq_to_map_upd (#k:eqtype) (#v:Type0) (s:Seq.seq (option (k & v)))
   (i:nat{i < Seq.length s})
   (x:k) (y:v)
   : Lemma
